Started proving a little bit.
Added dependency on Mathlib for linarith.

BkTree.lean
@@ -1,4 +1,7 @@
 import Lean
+import Mathlib.Tactic
+
+open Lean (AssocList)
 
 -- TODO: use a predefined metric class.
 class metric (α : Type _) :=
@@ -7,15 +10,14 @@ class metric (α : Type _) :=
 instance int_metric : metric Int where
   distance x y := Int.natAbs (x-y)
 
-def levenshtein (x' : List α) (y' : List α) [BEq α] : Nat :=
-  match x', y' with
+def levenshtein [BEq α]: (List α) → (List α) → Nat
   | [],[] => 0
   | [],y => y.length
   | x,[] => x.length
   | (x::xs),(y::ys) => if x == y then levenshtein xs ys
   else 1 + min3 (levenshtein xs (y::ys)) (levenshtein (x::xs) ys) (levenshtein xs ys)
 where min3 (a : Nat) (b : Nat) (c : Nat) : Nat := min (min a b) c
-termination_by levenshtein x y _ => x.length + y.length
+termination_by levenshtein _ x y => x.length + y.length
 
 instance levenshtein_metric {α: Type} [BEq α] : metric (List α) where
   distance x y := levenshtein x y
@@ -24,24 +26,25 @@ instance levenshtein_metric {α: Type} [BEq α] : metric (List α) where
 -- But doesn't matter too much until RBMap has split.
 inductive BkTree (β : Type _) (d : metric β) where
 | leaf
-| node (value : β) (children : (Lean.AssocList Nat (BkTree β d)))
+| node (value : β) (children : (AssocList Nat (BkTree β d)))
 deriving Inhabited
 
-def BkTree.size (t : BkTree β d) : Nat :=
-  match t with
+def BkTree.size : (BkTree β d) → Nat
   | leaf => 0
-  | node _ ts => foldl 1 ts
-where foldl : Nat → Lean.AssocList Nat (BkTree β d) → Nat
-      | n, Lean.AssocList.nil => n
-      | n, Lean.AssocList.cons _ v t => foldl (n + v.size) t
+  | node _ ts => foldl 0 ts
+where foldl : Nat → AssocList _ (BkTree β _) → Nat
+      | n, AssocList.nil => n
+      | n, AssocList.cons _ v t => foldl (n+1) t
+termination_by BkTree.size.foldl l => sizeOf l
 
-def BkTree.toList (t : BkTree β d) : List β :=
-  match t with
+def BkTree.toList : (BkTree β d) → List β
   | leaf => []
   | node v c => v::foldl [] c
-where foldl : List β → Lean.AssocList Nat (BkTree β d) → List β
-      | n, Lean.AssocList.nil => n
-      | n, Lean.AssocList.cons _ v t => foldl (n ++ v.toList) t
+where foldl : List β → AssocList _ (BkTree β _) → List β
+      | n, AssocList.nil => n
+      | n, AssocList.cons _ v t => foldl (n ++ v.toList) t
+termination_by BkTree.toList t => sizeOf t
+               BkTree.toList.foldl l => sizeOf l
 
 -- TODO: prove e.g. that `t.toList.length == t.size`
 
@@ -52,13 +55,12 @@ def BkTree.empty : BkTree β d :=
   BkTree.leaf
 
 def BkTree.singleton (v : β) : BkTree β d :=
-  BkTree.node v Lean.AssocList.nil
+  BkTree.node v AssocList.nil
 
 -- inserts a new element into a bk tree
-partial def BkTree.insert (t : BkTree β d) (v : β) : BkTree β d :=
-  match t with
-  | leaf => singleton v
-  | node val cs => 
+partial def BkTree.insert : (BkTree β d) → β → BkTree β d
+  | leaf, v => singleton v
+  | node val cs, v => 
     let dist := d.distance v val;
     if dist == 0 then (node val cs) 
     else match cs.find? dist with
@@ -66,25 +68,52 @@ partial def BkTree.insert (t : BkTree β d) (v : β) : BkTree β d :=
     | some c => node val (cs.replace dist (c.insert v))
 -- TODO: prove termination and remove `partial`.
 
+-- Thanks to Arthur Adjedj!
+theorem sizeof_assoclist_find [SizeOf α] [BEq α] [SizeOf β] {cs : AssocList α β } :
+  AssocList.find? d cs = some c → sizeOf c < 1 + sizeOf cs :=
+by
+  intro h
+  induction cs <;> simp at * <;>
+  rw [AssocList.find?] at *
+  . contradiction
+  . rename_i key value tail tail_ih
+    split at h
+    . cases h
+      linarith
+    . have : sizeOf c < 1 + sizeOf tail := tail_ih h
+      linarith
+
 -- checks if the BkTree contains an element
-partial def BkTree.contains (t : BkTree β d) (v : β) : Bool :=
-  match t with
-  | leaf => false
-  | node val cs =>
+def BkTree.contains : (BkTree β d) → (v : β) → Bool
+  | leaf, _ => false
+  | node val cs, v =>
     let dist := d.distance v val;
     if dist == 0 then true
-    else match cs.find? dist with
+    else match h: cs.find? dist with
     | none => false
     | some c => c.contains v
--- TODO: prove termination and remove `partial`.
+termination_by BkTree.contains t _ => sizeOf t
+decreasing_by {
+  simp_wf
+  exact sizeof_assoclist_find h
+}
 
 -- Returns a new AssocList that contains all elements with keys between min and max.
 -- TODO: generalize to work with any key [k : LE] instead of Nat. Gave a Prop instead of a Bool though..
 -- Would be more efficient if RBMap had .split but I think it doesn't.
-def Lean.AssocList.narrow (l : Lean.AssocList Nat c) (min: Nat) (max: Nat) : (Lean.AssocList Nat c) :=
-  match l with
-  | Lean.AssocList.nil => Lean.AssocList.nil
-  | Lean.AssocList.cons x y ls => if (min <= x) && (x <= max) then Lean.AssocList.cons x y (ls.narrow min max) else (ls.narrow min max)
+def Lean.AssocList.narrow : (AssocList Nat c) → Nat → Nat → (AssocList Nat c)
+  | AssocList.nil, _, _ => AssocList.nil
+  | AssocList.cons x y ls, min, max => if (min <= x) && (x <= max) then AssocList.cons x y (ls.narrow min max) else (ls.narrow min max)
+
+@[simp]
+theorem sizeof_assoclist_narrow [SizeOf β] {cs : AssocList Nat β } {min : Nat} {max : Nat} :
+  sizeOf cs ≥ sizeOf (cs.narrow min max) :=
+by
+  induction cs <;> rw [AssocList.narrow]
+  simp
+  split
+  simp_all
+  linarith
 
 -- Find all elements that are at most `dist` away from `v`.
 partial def BkTree.near (t : BkTree β d) (dist : Nat) (v : β) : (List β) :=
@@ -93,9 +122,11 @@ partial def BkTree.near (t : BkTree β d) (dist : Nat) (v : β) : (List β) :=
   | node val cs => 
   let d := d.distance v val;
   let sublist := cs.narrow (d-dist-1) (d+dist+1);
-  let subtrees := sublist.toList.map Prod.snd;
-  let rest := subtrees.foldl (fun x y => x ++ y.near dist v) []
+  let rest := foldl [] sublist
   if (d <= dist) then val::rest else rest
+where foldl : (List β) → AssocList _ (BkTree β _) → (List β)
+  | vs, AssocList.nil => vs
+  | vs, AssocList.cons _ y ls => foldl (vs ++ y.near dist v) ls
 -- TODO: prove termination and remove `partial`.
 
 partial def findClosest (v : β) (candidate : (β × Nat)) (t : BkTree β d) : (β × Nat) :=
